get fairly close to a sorry-free proof

Clean/Gadgets/Bits.lean
@@ -149,7 +149,7 @@ def circuit (n : ℕ) (hn : 2^n < p) : FormalCircuit (F p) field (BitVector n) w
   initial_offset_eq _ n := by simp only [main, circuit_norm]
   local_length_eq _ _ := by simp only [main, circuit_norm, Boolean.circuit]; ac_rfl
   output_eq _ _ := by
-    simp only [main, circuit_norm, Boolean.circuit, Circuit.forEach.apply_eq, var_from_offset_vector]
+    simp only [main, circuit_norm, Boolean.circuit, var_from_offset_vector]
 
   assumptions (x : F p) := x.val < 2^n
 
@@ -162,8 +162,11 @@ def circuit (n : ℕ) (hn : 2^n < p) : FormalCircuit (F p) field (BitVector n) w
     simp only [main, circuit_norm, Boolean.circuit, true_and, eval_vector, var_from_offset_vector] at *
     split at h_holds
     · rename_i h_eq
-      obtain rfl : n = 0 := Circuit.forEach.no_empty h_eq
-      simp [Vector.mapRange_zero]
+      rcases (Circuit.forEach.no_empty h_eq) with h|h
+      · obtain rfl : n = 0 := h
+        simp [Vector.mapRange_zero]
+      obtain ⟨_, _, h⟩ := h
+      exact Operations.noConfusion h
     rename_i h_eq; clear h_eq
     simp only [h_input, circuit_norm, subcircuit_norm, true_implies] at h_holds
     clear h_input
@@ -190,8 +193,11 @@ def circuit (n : ℕ) (hn : 2^n < p) : FormalCircuit (F p) field (BitVector n) w
     simp only [main, circuit_norm, Boolean.circuit, eval_vector, var_from_offset_vector] at *
     split
     · rename_i h_eq
-      obtain rfl : n = 0 := Circuit.forEach.no_empty h_eq
-      simp_all [Expression.eval, from_bits_expr]
+      rcases (Circuit.forEach.no_empty h_eq) with h|h
+      · obtain rfl : n = 0 := h
+        simp_all [Expression.eval, from_bits_expr]
+      obtain ⟨_, _, h⟩ := h
+      exact Operations.noConfusion h
     rename_i h_eq; clear h_eq
     simp only [h_input, circuit_norm, subcircuit_norm, true_implies, true_and, and_true] at h_env ⊢
     obtain ⟨ h_bits, right ⟩ := h_env; clear right;
